Unified ebfs

Original_Dinitz_Refine.thy
@@ -19,6 +19,7 @@ lemmas nfoldli_to_fold =
 
 (* TODO remove notation *)
 term Ref.update
+(*no_notation Ref.update ("_ := _")*)
 
 subsection \<open>Primitives\<close>
 definition deleteEdge :: "edge \<Rightarrow> _ graph \<Rightarrow> _ graph" where
@@ -27,6 +28,9 @@ definition deleteEdge :: "edge \<Rightarrow> _ graph \<Rightarrow> _ graph" wher
 text \<open>See EdmondsKarp_Impl.augment_edge\<close>
 definition subtractEdge :: "edge \<Rightarrow> ('capacity::linordered_idom) \<Rightarrow> _ graph \<Rightarrow> _ graph" where
   "subtractEdge e cap c \<equiv> c(e := c e - cap)"
+
+definition (in Graph) transferEdge :: "edge \<Rightarrow> _ graph \<Rightarrow> _ graph" where
+  "transferEdge e c' \<equiv> c'(e := c e)"
 \<comment> \<open>Primitives\<close>
 
 subsection \<open>Deleting a set of edges\<close>
@@ -538,10 +542,520 @@ qed
 \<comment> \<open>Cleaning\<close>
 
 
+subsection \<open>Extended BFS\<close>
+text \<open>In this section, we present an extended version of breadth-first search, which builds a graph
+      consisting of all shortest paths starting at a source node, instead of only a single shortest
+      path to a specified destination.
+
+      While we loosely follow the verified implementation of BFS developed for the implementation
+      of Edmonds-Karp, there are multiple significant differences. First, unlike standard BFS, we
+      care about the capacity of edges as we build a graph instead of a path. Second, we use two
+      working sets, since we need to distinguish between nodes in the graph that were added in the
+      current phase (which are still eligible edge endpoints) and older nodes. Third, the setup
+      based on a single predecessor for each node does not work here as we do not necessarily have
+      a tree.\<close>
+
+subsubsection \<open>Transferring edges to another graph\<close>
+context Graph
+begin
+definition transferEdges :: "edge set \<Rightarrow> _ graph \<Rightarrow> _ graph" where
+  "transferEdges S c' = (\<lambda>e. if e \<in> S then c e else c' e)"
+
+definition transferEdgesRefine :: "edge set \<Rightarrow> _ graph \<Rightarrow> _ graph nres" where
+  "transferEdgesRefine S c' \<equiv> foreach S (\<lambda>e c'. RETURN (transferEdge e c')) c'"
+
+lemma transferEdge_alt: "transferEdge e c' = (\<lambda>e'. if e' = e then c e' else c' e')"
+  unfolding transferEdge_def by fastforce
+
+definition transferEdgesRefineInvar :: "edge set \<Rightarrow> _ graph \<Rightarrow> edge set \<Rightarrow> _ graph \<Rightarrow> bool" where
+  "transferEdgesRefineInvar S c' it c'' \<equiv> c'' = (\<lambda>e. if e \<in> S - it then c e else c' e)"
+
+lemma transferEdgesRefine_correct:
+  "finite S \<Longrightarrow> transferEdgesRefine S c' \<le> RETURN (transferEdges S c')"
+  unfolding transferEdgesRefine_def transferEdges_def
+  apply (refine_vcg FOREACH_rule[where I="transferEdgesRefineInvar S c'"])
+  unfolding transferEdgesRefineInvar_def transferEdge_alt by fastforce+
+
+lemma transferEdges_capcomp:
+  "CapacityCompatibleGraphs c' c \<Longrightarrow> CapacityCompatibleGraphs (transferEdges S c') c"
+  unfolding transferEdges_def
+  by unfold_locales (simp add: CapacityCompatibleGraphs.cap_compatible)
+
+lemma transferEdges_E: "Graph.E (transferEdges S c') = Graph.E c' - S \<union> (S \<inter> E)"
+  unfolding Graph.E_def transferEdges_def by auto
+
+lemma transferEdges_ss_E: "S \<subseteq> E \<Longrightarrow> Graph.E (transferEdges S c') = Graph.E c' \<union> S"
+  using transferEdges_E by blast
+end
+
+interpretation transferEdges_dual:
+  Dual_Graph_Algorithms "Graph.transferEdgesRefine c S" "Graph.transferEdgesRefine (c\<^sup>T) (prod.swap ` S)" for c S
+  unfolding Graph.transferEdgesRefine_def
+  apply (intro Dual_Graph_AlgorithmsI)
+  apply (all \<open>refine_rcg FOREACH_refine_rcg[where \<alpha>="prod.swap"]\<close>)
+  by (auto simp: transpose_graph_rel_def Graph.transferEdge_def)
+\<comment> \<open>Transferring edges to another graph\<close>
+
+subsubsection \<open>Extended Breadth First Search phase\<close>
+
+text \<open>NOTE: For the correctness proofs, we need "V_i = Graph.V c' \<union> s", that is, we need to assure
+      that the source node is contained in this vertex set. This is a consequence of the graph
+      model, where nodes without edges cannot exists, which results in the graph being empty during
+      the first iteration even though s is within distance 0 of itself.
+      If we merely had "V_i = Graph.V c'" (making it unnecessary to pass V_i as a separate parameter),
+      then if there were a self loop of s, the first phase iteration would add s to the queue for
+      the next iteration (as it is an outgoing neighbor of s and not contained in the graph),
+      violating the invariant.\<close>
+
+context Graph
+begin
+(* TODO here we directly use the refined version of transferEdges, where in rightPass we first
+  use the abstract version and refine later. Unify! *)
+definition ebfsPhase :: "node set \<Rightarrow> _ graph \<Rightarrow> node set \<Rightarrow> (_ graph \<times> node set) nres" where
+  "ebfsPhase V\<^sub>i c' Q \<equiv> foreach Q
+    (\<lambda>u (c', Q'). do {
+      let S = E `` {u} - V\<^sub>i;
+      c' \<leftarrow> transferEdgesRefine ({u} \<times> S) c';
+      let Q' = Q' \<union> S;
+      RETURN (c', Q')
+    })
+    (c', {})"
+
+definition ebfsPhaseInvar :: "node \<Rightarrow> nat \<Rightarrow> _ graph \<Rightarrow> node set \<Rightarrow> (_ graph \<times> node set) \<Rightarrow> bool" where
+  "ebfsPhaseInvar s n c\<^sub>i Q \<equiv> \<lambda>(c', Q').
+    CapacityCompatibleGraphs c' c
+    \<and> Graph.E c' = Graph.E c\<^sub>i \<union> E \<inter> (exactDistNodes n s - Q) \<times> Q'
+    \<and> Q' = exactDistNodes (Suc n) s \<inter> E `` (exactDistNodes n s - Q)"
+
+lemma ebfsPhase_initial:
+  assumes "Bounded_Source_Shortest_Path_Union c' c s V n"
+  shows "ebfsPhaseInvar s n c' (exactDistNodes n s) (c', {})"
+  unfolding ebfsPhaseInvar_def
+proof (intro case_prodI conjI)
+  from assms interpret Bounded_Source_Shortest_Path_Union c' c s V n .
+  show "CapacityCompatibleGraphs c' c" by intro_locales
+qed (simp_all)
+
+lemma ebfs_phase_final:
+  assumes BSPU: "Bounded_Source_Shortest_Path_Union c\<^sub>i c s V n"
+    and INVAR: "ebfsPhaseInvar s n c\<^sub>i {} (c', Q')"
+  shows "Bounded_Source_Shortest_Path_Union c' c s V (Suc n) \<and> Q' = exactDistNodes (Suc n) s"
+proof
+  from INVAR have "CapacityCompatibleGraphs c' c"
+    and E'_EQ: "Graph.E c' = Graph.E c\<^sub>i \<union> E \<inter> exactDistNodes n s \<times> Q'"
+    and Q'_EQ: "Q' = exactDistNodes (Suc n) s \<inter> E `` exactDistNodes n s"
+    unfolding ebfsPhaseInvar_def by auto
+  then interpret CapacityCompatibleGraphs c' c by simp
+  from BSPU interpret g\<^sub>i: Bounded_Source_Shortest_Path_Union c\<^sub>i c s V n .
+
+  have "exactDistNodes (Suc n) s \<subseteq> E `` exactDistNodes n s"
+  proof
+    fix v
+    assume "v \<in> exactDistNodes (Suc n) s"
+    then obtain p where "isShortestPath s p v" "length p = Suc n" unfolding exactDistNodes_def
+      by (fastforce elim: obtain_shortest_path simp: isShortestPath_min_dist_def)
+    then obtain u p\<^sub>u where "isShortestPath s p\<^sub>u u" "length p\<^sub>u = n" "(u, v) \<in> E"
+      by (metis isShortestPath_min_dist_def min_dist_suc obtain_shortest_path connected_def)
+    then show "v \<in> E `` exactDistNodes n s" unfolding exactDistNodes_def isShortestPath_min_dist_def
+      using isPath_rtc connected_edgeRtc by fastforce
+  qed
+  with Q'_EQ show "Q' = exactDistNodes (Suc n) s" by blast
+  with E'_EQ have E'_EQ: "E' = g\<^sub>i.E' \<union> E \<inter> exactDistNodes n s \<times> exactDistNodes (Suc n) s"
+    by simp
+
+  show "Bounded_Source_Shortest_Path_Union c' c s V (Suc n)"
+  proof (unfold_locales, intro pair_set_eqI)
+    fix u v
+    assume "(u, v) \<in> E'"
+    then consider (OLD) "(u, v) \<in> g\<^sub>i.E'"
+      | (NEW) "(u, v) \<in> E \<inter> exactDistNodes n s \<times> exactDistNodes (Suc n) s"
+      using E'_EQ by blast
+    then show "(u, v) \<in> \<Union> {set p |p. \<exists>t. t \<in> V \<and> isShortestPath s p t \<and> length p \<le> Suc n}"
+    proof cases
+      case OLD
+      then have "(u, v) \<in> \<Union> {set p |p. \<exists>t. t \<in> V \<and> isShortestPath s p t \<and> length p \<le> n}"
+        by (simp add: g\<^sub>i.bounded_shortest_s_path_union)
+      then show ?thesis by fastforce
+    next
+      case NEW
+      then have "connected s u" "Suc (min_dist s u) = min_dist s v" "(u, v) \<in> E" "min_dist s v = Suc n"
+        unfolding exactDistNodes_def by auto
+      then obtain p where SP: "isShortestPath s (p @ [(u, v)]) v"
+        using obtain_shortest_path shortestPath_append_edge by meson
+      with \<open>min_dist s v = Suc n\<close> have "length p = n" unfolding isShortestPath_min_dist_def by simp
+      moreover note SP \<open>(u, v) \<in> E\<close>
+      ultimately show ?thesis using V_def by fastforce
+    qed
+  next
+    fix u v
+    assume "(u, v) \<in> \<Union> {set p |p. \<exists>t. t \<in> V \<and> isShortestPath s p t \<and> length p \<le> Suc n}"
+    then obtain t p where "(u, v) \<in> set p" "isShortestPath s p t" "length p \<le> Suc n" by blast
+    then obtain p' where SP: "isShortestPath s (p' @ [(u, v)]) v" and LEN: "length p' \<le> n"
+      by (fastforce dest: split_list split_shortest_path_around_edge)
+    then have "(u, v) \<in> E" by (simp add: isPath_append isShortestPath_def)
+    from LEN consider (LEN_LE) "length p' < n" | (LEN_EQ) "length p' = n" by linarith
+    then show "(u, v) \<in> E'"
+    proof cases
+      case LEN_LE
+      with \<open>(u, v) \<in> E\<close> have "length (p' @ [(u, v)]) \<le> n" "v \<in> V"
+        unfolding V_def by auto
+      with SP show ?thesis using E'_EQ unfolding g\<^sub>i.bounded_shortest_s_path_union by fastforce
+    next
+      case LEN_EQ
+      with SP have "v \<in> exactDistNodes (Suc n) s"
+        unfolding exactDistNodes_def isShortestPath_min_dist_def connected_def by auto
+      moreover from SP LEN_EQ have "u \<in> exactDistNodes n s"
+        using split_shortest_path unfolding exactDistNodes_def isShortestPath_min_dist_def connected_def
+        by fastforce
+      moreover note \<open>(u, v) \<in> E\<close>
+      ultimately show ?thesis using E'_EQ by blast
+    qed
+  qed
+qed
+
+context
+  fixes s
+  assumes FINITE_REACHABLE: "finite (reachableNodes s)"
+begin
+(* TODO necessary? *)
+(*
+lemma finite_if_spu(*[intro]*): "Source_Shortest_Path_Union c' c s T \<Longrightarrow> Finite_Graph c'"
+proof
+  assume "Source_Shortest_Path_Union c' c s T"
+  then interpret Source_Shortest_Path_Union c' c s T .
+  have "Graph.V c' \<subseteq> reachableNodes s"
+    unfolding reachableNodes_def using sg_connected_remains_base_connected by blast
+  then show "finite (Graph.V c')" using FINITE_REACHABLE finite_subset by blast
+qed
+*)
+
+lemma ebfs_phase_step:
+  assumes BSPU: "Bounded_Source_Shortest_Path_Union c\<^sub>i c s V n"
+    and Q: "u \<in> Q" "Q \<subseteq> exactDistNodes n s"
+    and INVAR: "ebfsPhaseInvar s n c\<^sub>i Q (c', Q')"
+  defines "S \<equiv> E `` {u} - (Graph.V c\<^sub>i \<union> {s})"
+  shows "transferEdgesRefine ({u} \<times> S) c' \<le> (spec c''. ebfsPhaseInvar s n c\<^sub>i (Q - {u}) (c'', Q' \<union> S))"
+proof -
+  from Q have "connected s u" unfolding exactDistNodes_def by blast
+  then have "E `` {u} \<subseteq> reachableNodes s"
+    unfolding reachableNodes_def using connected_append_edge by blast
+  with FINITE_REACHABLE have "finite S" unfolding S_def using finite_subset by blast
+  then have "transferEdgesRefine ({u} \<times> S) c' \<le> return (transferEdges ({u} \<times> S) c')"
+    using transferEdgesRefine_correct by simp
+  also have "... \<le> (spec c''. ebfsPhaseInvar s n c\<^sub>i (Q - {u}) (c'', Q' \<union> S))"
+    unfolding ebfsPhaseInvar_def
+  proof (clarify, refine_vcg)
+    from INVAR have "CapacityCompatibleGraphs c' c"
+      and E'_EQ: "Graph.E c' = Graph.E c\<^sub>i \<union> E \<inter> (exactDistNodes n s - Q) \<times> Q'"
+      and Q'_EQ: "Q' = exactDistNodes (Suc n) s \<inter> E `` (exactDistNodes n s - Q)"
+      unfolding ebfsPhaseInvar_def by auto
+    then interpret CapacityCompatibleGraphs c' c by simp
+
+    show "CapacityCompatibleGraphs (transferEdges ({u} \<times> S) c') c"
+      using \<open>CapacityCompatibleGraphs c' c\<close> transferEdges_capcomp by blast
+
+    interpret g\<^sub>i: Graph c\<^sub>i .
+    from Q have "E `` {u} \<subseteq> boundedReachableNodes (Suc n) s"
+      unfolding boundedReachableNodes_alt using exactDistNodes_reachable_ss by blast
+    with BSPU have S_alt: "S = exactDistNodes (Suc n) s \<inter> E `` {u}"
+      unfolding S_def exactDistNodes_alt using BSPU_V'_boundedReachable by blast
+    with Q Q'_EQ show "Q' \<union> S = exactDistNodes (Suc n) s \<inter> E `` (exactDistNodes n s - (Q - {u}))"
+      by blast
+
+    have "{u} \<times> S \<subseteq> E" unfolding S_def by blast
+    then have "Graph.E (transferEdges ({u} \<times> S) c') = g\<^sub>i.E \<union> E \<inter> ((exactDistNodes n s - Q) \<times> Q' \<union> {u} \<times> S)"
+      using transferEdges_ss_E E'_EQ by blast
+    also have "... = g\<^sub>i.E \<union> E \<inter> (exactDistNodes n s - (Q - {u})) \<times> (Q' \<union> S)"
+      unfolding S_alt Q'_EQ using Q by blast
+    finally show "Graph.E (transferEdges ({u} \<times> S) c') = g\<^sub>i.E \<union> E \<inter> (exactDistNodes n s - (Q - {u})) \<times> (Q' \<union> S)" .
+  qed
+  finally show ?thesis .
+qed
+
+lemma ebfs_phase_correct:
+  assumes BSPU: "Bounded_Source_Shortest_Path_Union c' c s V n"
+  shows "ebfsPhase (Graph.V c' \<union> {s}) c' (exactDistNodes n s) \<le> SPEC (\<lambda>(c'', Q'). Bounded_Source_Shortest_Path_Union c'' c s V (Suc n) \<and> Q' = exactDistNodes (Suc n) s)"
+  unfolding ebfsPhase_def
+  apply (refine_vcg FOREACH_rule[where I="ebfsPhaseInvar s n c'"])
+  using FINITE_REACHABLE finite_subset exactDistNodes_reachable_ss boundedReachableNodes_ss apply meson
+  using BSPU ebfsPhase_initial ebfs_phase_step ebfs_phase_final by simp_all
+end
+end
+
+\<comment> \<open>Extended Breadth First Search phase\<close>
+
+subsubsection \<open>Extended Breadth First Search Outer Loop\<close>
+context Graph
+begin
+(* TODO the n exists only for analysis purposes, can we remove it? *)
+(* TODO curry *)
+(* TODO update V\<^sub>i by adding Q instead of recomputing it *)
+definition ebfs :: "node \<Rightarrow> _ graph nres" where
+  "ebfs s \<equiv> do {
+    (c', _, _) \<leftarrow> WHILE\<^sub>T
+      (\<lambda>(_, Q, _). Q \<noteq> {})
+      (\<lambda>(c', Q, n). do {
+        let V\<^sub>i = Graph.V c' \<union> {s};
+        (c', Q') \<leftarrow> ebfsPhase V\<^sub>i c' Q;
+        RETURN (c', Q', Suc n)
+      })
+      ((\<lambda>_. 0), {s}, 0);
+    RETURN c'
+  }"
+
+definition ebfsInvar :: "node \<Rightarrow> (_ graph \<times> node set \<times> nat) \<Rightarrow> bool" where
+  "ebfsInvar s \<equiv> \<lambda>(c', Q, n).
+    Bounded_Source_Shortest_Path_Union c' c s V n
+    \<and> Q = exactDistNodes n s"
+
+lemma ebfs_final:
+  assumes INVAR: "ebfsInvar s (c', {}, n)"
+  shows "Source_Shortest_Path_Union c' c s V"
+proof -
+  from INVAR interpret Bounded_Source_Shortest_Path_Union c' c s V n unfolding ebfsInvar_def by blast
+
+  show ?thesis
+  proof (unfold_locales, intro equalityI subsetI)
+    fix e
+    assume "e \<in> \<Union> {set p |p. \<exists>t. t \<in> V \<and> isShortestPath s p t}"
+    then obtain p t where P: "e \<in> set p" "t \<in> V" "isShortestPath s p t" by blast
+    have "length p < n"
+    proof (rule ccontr)
+      assume "\<not> length p < n"
+      with P obtain p' u where "isShortestPath s p' u" "length p' = n"
+        using split_list_min_len split_shortest_path by (metis not_le)
+      then have "u \<in> exactDistNodes n s"
+        unfolding exactDistNodes_def isShortestPath_min_dist_def connected_def by auto
+      with INVAR show False unfolding ebfsInvar_def by simp
+    qed
+    with P show "e \<in> E'" using bounded_shortest_s_path_union by fastforce
+  qed (auto simp: bounded_shortest_s_path_union)
+qed
+
+context
+  fixes s
+  assumes FINITE_REACHABLE: "finite (reachableNodes s)"
+begin
+thm ebfs_phase_correct[OF FINITE_REACHABLE]
+thm greater_bounded_def
+term greater_bounded
+find_consts "('a \<times> 'b \<times> 'c) \<Rightarrow> 'c"
+value "(snd \<circ> snd) ((1::nat), (2::nat), (3::nat))"
+term inv_image
+term less_than_bool
+find_consts "(nat \<times> nat) set"
+thm greater_bounded_Suc_iff
+find_theorems "_ \<Longrightarrow> _ \<le> SPEC _"
+thm SPEC_rule
+find_theorems pathVertices reachableNodes
+find_theorems pathVertices isSimplePath
+thm pathVertices_fwd
+thm distinct_card
+find_theorems pathVertices length
+
+(* TODO fix this hot mess *)
+lemma ebfs_step:
+  assumes INVAR: "ebfsInvar s (c', Q, n)" and Q: "Q \<noteq> {}"
+  shows "ebfsPhase (Graph.V c' \<union> {s}) c' Q \<le> SPEC (\<lambda>(c'', Q'). ebfsInvar s (c'', Q', Suc n) \<and> Suc n \<le> card (reachableNodes s))"
+proof -
+  from INVAR have "ebfsPhase (Graph.V c' \<union> {s}) c' Q \<le> SPEC (\<lambda>(c'', Q'). Bounded_Source_Shortest_Path_Union c'' c s V (Suc n) \<and> Q' = exactDistNodes (Suc n) s)"
+    using ebfs_phase_correct[OF FINITE_REACHABLE] unfolding ebfsInvar_def by blast
+  also have "... \<le> SPEC (\<lambda>(c'', Q'). ebfsInvar s (c'', Q', Suc n) \<and> Suc n \<le> card (reachableNodes s))"
+  proof (auto simp: ebfsInvar_def)
+    from INVAR Q obtain p u where "isShortestPath s p u" "length p = n"
+      unfolding ebfsInvar_def exactDistNodes_def
+      using obtain_shortest_path isShortestPath_min_dist_def by simp metis
+    then have "card (set (pathVertices s p)) = Suc n" apply (auto dest!: shortestPath_is_simple simp: isSimplePath_def)
+      using length_pathVertices_eq distinct_card by fastforce (* TODO *)
+    with \<open>isShortestPath s p u\<close>[THEN shortestPath_is_path, THEN pathVertices_reachable] show "Suc n \<le> card (reachableNodes s)"
+      by (metis FINITE_REACHABLE card_mono)
+  qed
+  finally show ?thesis .
+qed
+
+theorem ebfs_correct: "ebfs s \<le> (spec c'. Source_Shortest_Path_Union c' c s V)"
+  unfolding ebfs_def
+  apply (refine_vcg WHILET_rule[where I="ebfsInvar s"
+      and R="inv_image (greater_bounded (card (reachableNodes s))) (snd \<circ> snd)"])
+
+  apply blast
+
+  subgoal
+    unfolding ebfsInvar_def exactDistNodes_def
+    apply auto
+    apply unfold_locales
+    unfolding Graph.E_def
+    by auto
+
+  using ebfs_step ebfs_final by simp_all
+end
+end
+\<comment> \<open>Extended Breadth First Search Outer Loop\<close>
+
+subsubsection \<open>Backward EBFS\<close>
+context Graph
+begin
+definition ebfsBackward :: "node \<Rightarrow> _ graph nres" where
+  "ebfsBackward t \<equiv> do {
+    (c', _, _) \<leftarrow> WHILE\<^sub>T
+      (\<lambda>(_, Q, _). Q \<noteq> {})
+      (\<lambda>(c', Q, n). do {
+        let V\<^sub>i = (Graph.V c' \<union> {t});
+        (c', Q') \<leftarrow> foreach Q
+          (\<lambda>u (c', Q'). do {
+            let S = E\<inverse> `` {u} - V\<^sub>i;
+            c' \<leftarrow> transferEdgesRefine (S \<times> {u}) c';
+            let Q' = Q' \<union> S;
+            RETURN (c', Q')
+          })
+          (c', {});
+        RETURN (c', Q', Suc n)
+      })
+      ((\<lambda>_. 0), {t}, 0);
+    RETURN c'
+  }"
 
 
+(* TODO improve *)
+lemma dual_ebfs: "Dual_Graph_Algorithms (swap_args2 Graph.ebfsBackward u) (swap_args2 Graph.ebfs u)"
+proof (intro Dual_Graph_AlgorithmsI, unfold swap_args2_def)
+  fix c' :: "('capacity'::linordered_idom) graph"
+  note[refine_dref_RELATES] = RELATESI[of transpose_graph_rel]
+  show "Graph.ebfsBackward c' u \<le> \<Down> transpose_graph_rel (Graph.ebfs (c'\<^sup>T) u)"
+    unfolding Graph.ebfsBackward_def Graph.ebfs_def Graph.ebfsPhase_def
+    apply (refine_rcg FOREACH_refine_rcg[where \<alpha>=id], refine_dref_type)
+            apply (all \<open>(auto simp: transpose_graph_rel_def; fail)?\<close>)
+    apply (simp add: transferEdges_dual.conc_simp)
+    by (simp add: transpose_graph_rel_def product_swap)
 
+  show "Graph.ebfs c' u \<le> \<Down> transpose_graph_rel (Graph.ebfsBackward (c'\<^sup>T) u)"
+    unfolding Graph.ebfsBackward_def Graph.ebfs_def Graph.ebfsPhase_def
+    apply (refine_rcg FOREACH_refine_rcg[where \<alpha>=id])
+            apply refine_dref_type
+            apply (all \<open>(auto simp: transpose_graph_rel_def; fail)?\<close>)
+    apply (simp add: transferEdges_dual.conc_simp)
+    by (simp add: transpose_graph_rel_def product_swap)
+qed
 
+(* TODO simplify and extract *)
+lemma dual_spu: "Target_Shortest_Path_Union c' c (Graph.V c) t = Source_Shortest_Path_Union (c'\<^sup>T) (c\<^sup>T) t (Graph.V (c\<^sup>T))"
+proof
+  assume "Target_Shortest_Path_Union c' c (Graph.V c) t"
+  then interpret spu: Target_Shortest_Path_Union c' c "Graph.V c" t .
+  show "Source_Shortest_Path_Union (c'\<^sup>T) (c\<^sup>T) t (Graph.V (c\<^sup>T))"
+  proof
+    show "\<And>u v. (c'\<^sup>T) (u, v) = 0 \<or> (c\<^sup>T) (u, v) = 0 \<or> (c'\<^sup>T) (u, v) = (c\<^sup>T) (u, v)"
+      using spu.cap_compatible by simp
+    show "Graph.E (c'\<^sup>T) = \<Union> {set p |p. \<exists>ta. ta \<in> Graph.V (c\<^sup>T) \<and> Graph.isShortestPath (c\<^sup>T) t p ta}"
+    proof (simp, intro pair_set_eqI)
+      fix u v
+      assume "(u, v) \<in> spu.E'\<inverse>"
+      then obtain s p where "(v, u) \<in> set p" "s \<in> V" "isShortestPath s p t"
+        using spu.shortest_t_path_union by blast
+      then have "(u, v) \<in> set (transpose_path p)" "isShortestPath s (transpose_path (transpose_path p)) t"
+        by auto
+      with \<open>s \<in> V\<close> show "(u, v) \<in> \<Union> {set p |p. \<exists>ta. ta \<in> V \<and> isShortestPath ta (transpose_path p) t}"
+        by blast
+    next
+      fix u v
+      assume "(u, v) \<in> \<Union> {set p |p. \<exists>ta. ta \<in> V \<and> isShortestPath ta (transpose_path p) t}"
+      then show "(u, v) \<in> spu.E'\<inverse>" using spu.shortest_t_path_union by fastforce
+    qed
+  qed
+next
+  assume "Source_Shortest_Path_Union (c'\<^sup>T) (c\<^sup>T) t (Graph.V (c\<^sup>T))"
+  then interpret spu: Source_Shortest_Path_Union "c'\<^sup>T" "c\<^sup>T" t "Graph.V c" by simp
+  show "Target_Shortest_Path_Union c' c (Graph.V c) t"
+  proof
+    show "\<And>u v. c' (u, v) = 0 \<or> c (u, v) = 0 \<or> c' (u, v) = c (u, v)"
+      using spu.cap_compatible by simp
+    show "Graph.E c' = \<Union> {set p |p. \<exists>s. s \<in> Graph.V c \<and> Graph.isShortestPath c s p t}"
+    proof (intro pair_set_eqI)
+      fix u v
+      assume "(u, v) \<in> Graph.E c'"
+      then obtain s p where "(v, u) \<in> set p" "s \<in> V" "spu.isShortestPath t p s"
+        using spu.shortest_s_path_union by fastforce
+      then show "(u, v) \<in> \<Union> {set p |p. \<exists>s. s \<in> Graph.V c \<and> Graph.isShortestPath c s p t}"
+        by fastforce
+    next
+      fix u v
+      assume "(u, v) \<in> \<Union> {set p |p. \<exists>s. s \<in> Graph.V c \<and> Graph.isShortestPath c s p t}"
+      then obtain s p where "(u, v) \<in> set p" "s \<in> Graph.V c" "Graph.isShortestPath c s p t"
+        by blast
+      then have "(v, u) \<in> set (transpose_path p)" "spu.isShortestPath t (transpose_path p) s" by auto
+      with \<open>s \<in> Graph.V c\<close> have "(v, u) \<in> spu.E'" using spu.shortest_s_path_union by blast
+      then show "(u, v) \<in> Graph.E c'" by simp
+    qed
+  qed
+qed
+
+theorem (in Graph) ebfsBackward_correct:
+  assumes FINITE_REACHED_FROM: "finite {u. connected u t}"
+  shows "ebfsBackward t \<le> (spec c'. Target_Shortest_Path_Union c' c V t)"
+proof -
+  interpret Dual_Graph_Algorithms "swap_args2 Graph.ebfsBackward t" "swap_args2 Graph.ebfs t"
+    using dual_ebfs .
+  have "swap_args2 Graph.ebfsBackward t c \<le> (spec c'. Target_Shortest_Path_Union c' c V t)"
+    (*using dual_spu apply (auto elim!: transfer_spec)*)
+    (*thm dual_spu[THEN transfer_spec]*)
+    (*thm transfer_spec[OF dual_spu]*)
+  proof (intro transfer_spec[where spec'="\<lambda>c c'. Source_Shortest_Path_Union c' c t (Graph.V c)"])
+    show "\<And>c c'. Target_Shortest_Path_Union c' c (Graph.V c) t = Source_Shortest_Path_Union (c'\<^sup>T) (c\<^sup>T) t (Graph.V (c\<^sup>T))"
+      using Graph.dual_spu .
+    thm Graph.ebfs_correct
+    from FINITE_REACHED_FROM have "finite (Graph.reachableNodes (c\<^sup>T) t)"
+      unfolding Graph.reachableNodes_def by simp
+    then show "swap_args2 Graph.ebfs t (c\<^sup>T) \<le> (spec c'. Source_Shortest_Path_Union c' (c\<^sup>T) t (Graph.V (c\<^sup>T)))"
+      using Graph.ebfs_correct by fastforce
+  qed
+  then show ?thesis by simp
+qed
+end
+\<comment> \<open>Backward EBFS\<close>
+
+subsubsection \<open>Building a dual layering\<close>
+context Graph
+begin
+(* TODO bounded version *)
+definition buildDualLayering :: "node \<Rightarrow> node \<Rightarrow> _ graph nres" where
+  "buildDualLayering s t \<equiv> do {
+    sl \<leftarrow> ebfs s;
+    stl \<leftarrow> Graph.ebfsBackward sl t;
+    RETURN stl
+  }"
+end
+
+(* TODO is Finite_Graph really what we want? *)
+context Finite_Graph
+begin
+lemma buildDualLayering_correct:
+  "buildDualLayering s t \<le> (spec c'. Dual_Shortest_Path_Union c' c s t)"
+  unfolding buildDualLayering_def
+proof (refine_vcg, simp)
+  have "reachableNodes s \<subseteq> V \<union> {s}"
+    using Graph.distinct_nodes_in_V_if_connected(2) reachableNodes_def by auto
+  then have "finite (reachableNodes s)" using finite_V by (simp add: finite_subset)
+  then have "ebfs s \<le> (spec sl. Source_Shortest_Path_Union sl c s V)" by (rule ebfs_correct)
+  also have "... \<le> (spec sl. Graph.ebfsBackward sl t \<le> (spec c'. Dual_Shortest_Path_Union c' c s t))"
+  proof (rule SPEC_rule)
+    fix c'
+    assume "Source_Shortest_Path_Union c' c s V"
+    then interpret Source_Shortest_Path_Union c' c s V .
+
+    have "{u. g'.connected u t} \<subseteq> V' \<union> {t}"
+      using g'.distinct_nodes_in_V_if_connected by auto
+    then have "finite {u. g'.connected u t}" using finite_V V_ss by (simp add: finite_subset)
+    then have "g'.ebfsBackward t \<le> (spec c''. Target_Shortest_Path_Union c'' c' V' t)"
+      by (rule g'.ebfsBackward_correct)
+    also from \<open>Source_Shortest_Path_Union c' c s V\<close> have "... \<le> (spec c''. Dual_Shortest_Path_Union c'' c s t)"
+      using SPEC_rule ST_SPU_dualI by metis
+    finally show "g'.ebfsBackward t \<le> (spec c''. Dual_Shortest_Path_Union c'' c s t)" .
+  qed
+  finally show "ebfs s \<le> (spec sl. Graph.ebfsBackward sl t \<le> (spec c'. Dual_Shortest_Path_Union c' c s t))" .
+qed
+end
+\<comment> \<open>Building a dual layering\<close>
+\<comment> \<open>Extended BFS\<close>
 
 
 
@@ -569,47 +1083,7 @@ qed
 
 
 subsection \<open>Dinitz phase refinement\<close>
-context Graph
-begin
-(* TODO bounded version *)
-definition build_st_layering :: "node \<Rightarrow> node \<Rightarrow> _ graph nres" where
-  "build_st_layering s t \<equiv> do {
-    sl \<leftarrow> ebfs s;
-    stl \<leftarrow> Graph.back_ebfs sl t;
-    RETURN stl
-  }"
-end
 
-(* TODO is Finite_Graph really what we want? *)
-context Finite_Graph
-begin
-lemma build_st_layering_correct:
-  "build_st_layering s t \<le> (spec c'. Dual_Shortest_Path_Union c' c s t)"
-  unfolding build_st_layering_def
-proof (refine_vcg, simp)
-  have "reachableNodes s \<subseteq> V \<union> {s}"
-    using Graph.distinct_nodes_in_V_if_connected(2) reachableNodes_def by auto
-  then have "finite (reachableNodes s)" using finite_V by (simp add: finite_subset)
-  then have "ebfs s \<le> (spec sl. Source_Shortest_Path_Union sl c s V)" by (rule ebfs_correct)
-  also have "... \<le> (spec sl. Graph.back_ebfs sl t \<le> (spec c'. Dual_Shortest_Path_Union c' c s t))"
-  proof (rule SPEC_rule)
-    fix c'
-    assume "Source_Shortest_Path_Union c' c s V"
-    then interpret Source_Shortest_Path_Union c' c s V .
-
-    have "{u. g'.connected u t} \<subseteq> V' \<union> {t}"
-      using g'.distinct_nodes_in_V_if_connected by auto
-    then have "finite {u. g'.connected u t}" using finite_V V_ss by (simp add: finite_subset)
-    then have "g'.back_ebfs t \<le> (spec c''. Target_Shortest_Path_Union c'' c' V' t)"
-      by (rule g'.back_ebfs_correct)
-    also from \<open>Source_Shortest_Path_Union c' c s V\<close> have "... \<le> (spec c''. Dual_Shortest_Path_Union c'' c s t)"
-      using SPEC_rule ST_SPU_dualI by metis
-    finally show "g'.back_ebfs t \<le> (spec c''. Dual_Shortest_Path_Union c'' c s t)" .
-  qed
-  finally show "ebfs s \<le> (spec sl. Graph.back_ebfs sl t \<le> (spec c'. Dual_Shortest_Path_Union c' c s t))" .
-qed
-
-end
 
 
 
